more proof abstract

src/BinEncoders/Env/Examples/Dns.v
@@ -18,7 +18,19 @@ Require Import
         Fiat.BinEncoders.Env.Lib.SteppingCacheList.
 
 Set Implicit Arguments.
+
 Notation compose := Fiat.BinEncoders.Env.Common.Compose.compose.
+Notation "x 'Then' y" := (compose btransformer x y) (at level 100, right associativity).
+Notation "x 'Done'"   := (x Then fun e => (nil, e)) (at level 99, right associativity).
+Notation "[ n ]" := (exist _ n _).
+
+Arguments Bool_encode {_ _} _ _.
+Arguments Char_encode {_ _} _ _.
+Arguments FixInt_encode {_ _ _} _ _.
+Arguments Enum_encode {_ _ _ _} _ _ _.
+Arguments FixList_encode {_ _ _} _ _ _ _.
+Arguments IList_encode {_ _ _} _ _ _ _.
+Arguments SteppingList_encode {_ _ _ _ _ _ _} _ {_} _ _ _ _ _.
 
 Inductive type_t := A | CNAME | NS | MX.
 Inductive class_t := IN | CH | HS.
@@ -58,35 +70,24 @@ Record packet_t :=
 
 Definition FixInt_of_branch (b : CacheBranch) : {n | (n < exp2 2)%N}.
   refine (match b with
-          | Yes => exist _ (3%N) _
-          | No  => exist _ (0%N) _
+          | Yes => [3%N]
+          | No  => [0%N]
           end); abstract (rewrite <- N.compare_lt_iff; eauto).  Defined.
 
 Definition FixInt_of_type (t : type_t) : {n | (n < exp2 16)%N}.
   refine (match t with
-          | A     => exist _ (1%N) _
-          | CNAME => exist _ (5%N) _
-          | NS    => exist _ (2%N) _
-          | MX    => exist _ (15%N) _
+          | A     => [1%N]
+          | CNAME => [5%N]
+          | NS    => [2%N]
+          | MX    => [15%N]
           end); abstract (rewrite <- N.compare_lt_iff; eauto).  Defined.
 
 Definition FixInt_of_class (c : class_t) : {n | (n < exp2 16)%N}.
   refine (match c with
-          | IN => exist _ (1%N) _
-          | CH => exist _ (3%N) _
-          | HS => exist _ (4%N) _
+          | IN => [1%N]
+          | CH => [3%N]
+          | HS => [4%N]
           end); abstract (rewrite <- N.compare_lt_iff; eauto).  Defined.
-
-Notation "x 'Then' y" := (compose btransformer x y) (at level 100, right associativity).
-Notation "x 'Done'"   := (x Then fun e => (nil, e)) (at level 99, right associativity).
-
-Arguments Bool_encode {_ _} _ _.
-Arguments Char_encode {_ _} _ _.
-Arguments FixInt_encode {_ _ _} _ _.
-Arguments Enum_encode {_ _ _ _} _ _ _.
-Arguments FixList_encode {_ _ _} _ _ _ _.
-Arguments IList_encode {_ _ _} _ _ _ _.
-Arguments SteppingList_encode {_ _ _ _ _ _ _} _ {_} _ _ _ _ _.
 
 Definition encode_word (w : word_t) :=
        FixInt_encode (FixList_getlength w.(word))
@@ -133,8 +134,7 @@ Proof. solve_decoder.  Defined.
 Definition empty :=
   {| eMap := EMap.empty _;
      dMap := DMap.empty _;
-     tick := 0;
-     extr := 0 |}.
+     offs := 0 |}.
 
 Lemma empty_Equiv : Equiv empty empty.
 Proof.
@@ -169,6 +169,25 @@ Proof.
   specialize (H eq_refl eq_refl).
   intuition.  Qed.
 
+Section Examples.
+  Definition packet_uncompressed :=
+    true :: true :: false :: true :: true :: false :: true :: true :: false :: true :: false :: false :: false :: false :: true :: false :: false :: false :: false :: false :: false :: false :: false :: true :: false :: false :: false :: false :: false :: false :: false :: false :: false :: false :: false :: false :: false :: false :: false :: false :: false :: false :: false :: false :: false :: false :: false :: true :: false :: false :: false :: false :: false :: false :: false :: false :: false :: false :: false :: false :: false :: false :: false :: false :: false :: false :: false :: false :: false :: false :: false :: false :: false :: false :: false :: false :: false :: false :: false :: false :: false :: false :: false :: false :: false :: false :: false :: false :: false :: false :: false :: false :: false :: false :: false :: false :: false :: false :: false :: false :: false :: false :: true :: true :: false :: true :: true :: true :: false :: true :: true :: true :: false :: true :: true :: true :: false :: true :: true :: true :: false :: true :: true :: true :: false :: true :: true :: true :: false :: false :: false :: false :: true :: true :: false :: false :: false :: true :: true :: false :: true :: true :: true :: false :: false :: true :: true :: false :: true :: true :: true :: true :: false :: true :: true :: true :: false :: false :: true :: false :: false :: true :: true :: true :: false :: true :: false :: false :: false :: true :: true :: false :: true :: false :: false :: false :: false :: true :: true :: false :: false :: true :: false :: true :: false :: true :: true :: false :: false :: false :: false :: true :: false :: true :: true :: true :: false :: false :: true :: true :: false :: true :: true :: true :: false :: true :: false :: false :: false :: true :: true :: false :: false :: true :: false :: true :: false :: true :: true :: true :: false :: false :: true :: false :: false :: true :: true :: false :: true :: true :: true :: false :: false :: false :: false :: false :: false :: false :: true :: true :: false :: true :: true :: false :: false :: true :: false :: true :: false :: true :: true :: false :: false :: true :: false :: false :: false :: true :: true :: true :: false :: true :: false :: true :: false :: false :: false :: false :: false :: false :: false :: false :: false :: false :: false :: false :: false :: false :: false :: false :: false :: false :: false :: false :: false :: false :: false :: true :: false :: false :: false :: false :: false :: false :: false :: false :: false :: false :: false :: false :: false :: false :: false :: true :: nil.
+  Definition packet_compressed :=
+    true :: true :: false :: true :: true :: false :: true :: true :: false :: true :: false :: false :: false :: false :: true :: false :: true :: false :: false :: false :: false :: false :: false :: true :: true :: false :: false :: false :: false :: false :: false :: false :: false :: false :: false :: false :: false :: false :: false :: false :: false :: false :: false :: false :: false :: false :: false :: true :: false :: false :: false :: false :: false :: false :: false :: false :: false :: false :: false :: false :: false :: false :: false :: true :: false :: false :: false :: false :: false :: false :: false :: false :: false :: false :: false :: false :: false :: false :: false :: false :: false :: false :: false :: false :: false :: false :: false :: false :: false :: false :: false :: false :: false :: false :: false :: false :: false :: false :: false :: false :: false :: false :: true :: true :: false :: true :: true :: true :: false :: true :: true :: true :: false :: true :: true :: true :: false :: true :: true :: true :: false :: true :: true :: true :: false :: true :: true :: true :: false :: false :: false :: false :: true :: true :: false :: false :: false :: true :: true :: false :: true :: true :: true :: false :: false :: true :: true :: false :: true :: true :: true :: true :: false :: true :: true :: true :: false :: false :: true :: false :: false :: true :: true :: true :: false :: true :: false :: false :: false :: true :: true :: false :: true :: false :: false :: false :: false :: true :: true :: false :: false :: true :: false :: true :: false :: true :: true :: false :: false :: false :: false :: true :: false :: true :: true :: true :: false :: false :: true :: true :: false :: true :: true :: true :: false :: true :: false :: false :: false :: true :: true :: false :: false :: true :: false :: true :: false :: true :: true :: true :: false :: false :: true :: false :: false :: true :: true :: false :: true :: true :: true :: false :: false :: false :: false :: false :: false :: false :: true :: true :: false :: true :: true :: false :: false :: true :: false :: true :: false :: true :: true :: false :: false :: true :: false :: false :: false :: true :: true :: true :: false :: true :: false :: true :: false :: false :: false :: false :: false :: false :: false :: false :: false :: false :: false :: false :: false :: false :: false :: false :: false :: false :: false :: false :: false :: false :: false :: true :: false :: false :: false :: false :: false :: false :: false :: false :: false :: false :: false :: false :: false :: false :: false :: true :: true :: true :: false :: false :: false :: false :: false :: false :: false :: false :: false :: false :: true :: true :: false :: false :: false :: false :: false :: false :: false :: false :: false :: false :: false :: false :: false :: false :: false :: false :: false :: true :: false :: false :: false :: false :: false :: false :: false :: false :: false :: false :: false :: false :: false :: false :: false :: true :: false :: false :: false :: false :: false :: false :: false :: false :: false :: false :: false :: false :: false :: false :: false :: false :: false :: false :: false :: false :: false :: false :: true :: false :: false :: true :: false :: true :: true :: false :: false :: false :: false :: false :: false :: false :: false :: false :: false :: false :: false :: false :: false :: false :: false :: true :: false :: false :: true :: false :: false :: true :: true :: false :: true :: true :: false :: false :: true :: false :: false :: false :: false :: true :: false :: false :: false :: true :: false :: false :: false :: true :: false :: true :: false :: false :: false :: true :: false :: false :: nil.
+End Examples.
+
+Goal True.
+  pose (packet_decode packet_uncompressed) as goal.
+  unfold packet_decode in goal.
+  (* Time simpl in goal. (* ~ 100 seconds *) *)
+Abort.
+
+(*
+Goal True.
+  pose (packet_decode packet_compressed) as goal.
+  unfold packet_decode in goal.
+  Time simpl in goal.
+Abort. *)
 
 Extract Inductive bool => "bool" [ "true" "false" ].
 Extract Inductive nat => "int"
@@ -182,16 +201,7 @@ Extract Inductive ascii => char [
 ]
 "(fun f c -> let n = Char.code c in let h i = (n land (1 lsl i)) <> 0 in f (h 0) (h 1) (h 2) (h 3) (h 4) (h 5) (h 6) (h 7))".
 
-Section Examples.
-
-  Definition packet_uncompressed :=
-    true :: true :: false :: true :: true :: false :: true :: true :: false :: true :: false :: false :: false :: false :: true :: false :: false :: false :: false :: false :: false :: false :: false :: true :: false :: false :: false :: false :: false :: false :: false :: false :: false :: false :: false :: false :: false :: false :: false :: false :: false :: false :: false :: false :: false :: false :: false :: true :: false :: false :: false :: false :: false :: false :: false :: false :: false :: false :: false :: false :: false :: false :: false :: false :: false :: false :: false :: false :: false :: false :: false :: false :: false :: false :: false :: false :: false :: false :: false :: false :: false :: false :: false :: false :: false :: false :: false :: false :: false :: false :: false :: false :: false :: false :: false :: false :: false :: false :: false :: false :: false :: false :: true :: true :: false :: true :: true :: true :: false :: true :: true :: true :: false :: true :: true :: true :: false :: true :: true :: true :: false :: true :: true :: true :: false :: true :: true :: true :: false :: false :: false :: false :: true :: true :: false :: false :: false :: true :: true :: false :: true :: true :: true :: false :: false :: true :: true :: false :: true :: true :: true :: true :: false :: true :: true :: true :: false :: false :: true :: false :: false :: true :: true :: true :: false :: true :: false :: false :: false :: true :: true :: false :: true :: false :: false :: false :: false :: true :: true :: false :: false :: true :: false :: true :: false :: true :: true :: false :: false :: false :: false :: true :: false :: true :: true :: true :: false :: false :: true :: true :: false :: true :: true :: true :: false :: true :: false :: false :: false :: true :: true :: false :: false :: true :: false :: true :: false :: true :: true :: true :: false :: false :: true :: false :: false :: true :: true :: false :: true :: true :: true :: false :: false :: false :: false :: false :: false :: false :: true :: true :: false :: true :: true :: false :: false :: true :: false :: true :: false :: true :: true :: false :: false :: true :: false :: false :: false :: true :: true :: true :: false :: true :: false :: true :: false :: false :: false :: false :: false :: false :: false :: false :: false :: false :: false :: false :: false :: false :: false :: false :: false :: false :: false :: false :: false :: false :: false :: true :: false :: false :: false :: false :: false :: false :: false :: false :: false :: false :: false :: false :: false :: false :: false :: true :: nil.
-
-
-  Definition packet_compressed :=
-    true :: true :: false :: true :: true :: false :: true :: true :: false :: true :: false :: false :: false :: false :: true :: false :: true :: false :: false :: false :: false :: false :: false :: true :: true :: false :: false :: false :: false :: false :: false :: false :: false :: false :: false :: false :: false :: false :: false :: false :: false :: false :: false :: false :: false :: false :: false :: true :: false :: false :: false :: false :: false :: false :: false :: false :: false :: false :: false :: false :: false :: false :: false :: true :: false :: false :: false :: false :: false :: false :: false :: false :: false :: false :: false :: false :: false :: false :: false :: false :: false :: false :: false :: false :: false :: false :: false :: false :: false :: false :: false :: false :: false :: false :: false :: false :: false :: false :: false :: false :: false :: false :: true :: true :: false :: true :: true :: true :: false :: true :: true :: true :: false :: true :: true :: true :: false :: true :: true :: true :: false :: true :: true :: true :: false :: true :: true :: true :: false :: false :: false :: false :: true :: true :: false :: false :: false :: true :: true :: false :: true :: true :: true :: false :: false :: true :: true :: false :: true :: true :: true :: true :: false :: true :: true :: true :: false :: false :: true :: false :: false :: true :: true :: true :: false :: true :: false :: false :: false :: true :: true :: false :: true :: false :: false :: false :: false :: true :: true :: false :: false :: true :: false :: true :: false :: true :: true :: false :: false :: false :: false :: true :: false :: true :: true :: true :: false :: false :: true :: true :: false :: true :: true :: true :: false :: true :: false :: false :: false :: true :: true :: false :: false :: true :: false :: true :: false :: true :: true :: true :: false :: false :: true :: false :: false :: true :: true :: false :: true :: true :: true :: false :: false :: false :: false :: false :: false :: false :: true :: true :: false :: true :: true :: false :: false :: true :: false :: true :: false :: true :: true :: false :: false :: true :: false :: false :: false :: true :: true :: true :: false :: true :: false :: true :: false :: false :: false :: false :: false :: false :: false :: false :: false :: false :: false :: false :: false :: false :: false :: false :: false :: false :: false :: false :: false :: false :: false :: true :: false :: false :: false :: false :: false :: false :: false :: false :: false :: false :: false :: false :: false :: false :: false :: true :: true :: true :: false :: false :: false :: false :: false :: false :: false :: false :: false :: false :: true :: true :: false :: false :: false :: false :: false :: false :: false :: false :: false :: false :: false :: false :: false :: false :: false :: false :: false :: true :: false :: false :: false :: false :: false :: false :: false :: false :: false :: false :: false :: false :: false :: false :: false :: true :: false :: false :: false :: false :: false :: false :: false :: false :: false :: false :: false :: false :: false :: false :: false :: false :: false :: false :: false :: false :: false :: false :: true :: false :: false :: true :: false :: true :: true :: false :: false :: false :: false :: false :: false :: false :: false :: false :: false :: false :: false :: false :: false :: false :: false :: true :: false :: false :: true :: false :: false :: true :: true :: false :: true :: true :: false :: false :: true :: false :: false :: false :: false :: true :: false :: false :: false :: true :: false :: false :: false :: true :: false :: true :: false :: false :: false :: true :: false :: false :: nil.
-
-End Examples.
+(* Extraction "dns.ml" packet_encode packet_decode packet_uncompressed packet_compressed. *)
 
 (*
 #use "dns.ml";;
@@ -199,295 +209,4 @@ packet_decode packet_uncompressed;;
 packet_decode packet_compressed;;
 let p = packet_decode packet_uncompressed;;
 let q = {pid = pid p; pmask = pmask p; pquestion = pquestion p; panswer = [{rname = qname (List.hd (pquestion p)); rtype = A; rclass = IN; rttl = Npos XH; rdata = []}]; pauthority = []; padditional = []};;
-*)
-
-(* Extraction "dns.ml" packet_encode packet_decode packet_uncompressed packet_compressed. *)
-
-(*
-  Notation "[ n ]" := (exist _ n _).
-  Definition ans := fst (fst (decode (decoder:=FixInt_decoder (size:=5) _ (fun _ => True))
-                                     packet_uncompressed empty)).
-
-(*  Instance cahceFakeAdd : CacheAdd cache nat :=
-    {| addE := fun e _ => e;
-       addD := fun e _ => e; |}.
-  Proof. abstract (unfold Equiv; eauto).  Qed. *)
-
-
-Instance cacheAddNat2 : CacheAdd cache nat :=
-  {| addE := fun c n => cycle n (fun c => if PeanoNat.Nat.eqb 0 c.(extr)
-                                          then {| eMap := c.(eMap);
-                                                  dMap := c.(dMap);
-                                                  tick := 1 + c.(tick);
-                                                  extr := 0 |}
-                                          else {| eMap := c.(eMap);
-                                                  dMap := c.(dMap);
-                                                  tick := c.(tick);
-                                                  extr := 1 + c.(extr) |}) c;
-     addD := fun c n => cycle n (fun c => if PeanoNat.Nat.eqb 0 c.(extr)
-                                          then {| eMap := c.(eMap);
-                                                  dMap := c.(dMap);
-                                                  tick := 1 + c.(tick);
-                                                  extr := 0 |}
-                                          else {| eMap := c.(eMap);
-                                                  dMap := c.(dMap);
-                                                  tick := c.(tick);
-                                                  extr := 1 + c.(extr) |}) c; |}.
-Proof.
-  admit.  Defined.
-
-(*
-  Instance cacheAddNatNoob : CacheAdd cache nat :=
-    {| addE := fun c n => cycle n (fun c => {| eMap := c.(eMap);
-                                               dMap := c.(dMap);
-                                               tick := 1 + c.(tick);
-                                               extr := 0 |}) c;
-       addD := fun c n => cycle n (fun c => {| eMap := c.(eMap);
-                                                    dMap := c.(dMap);
-                                                    tick := 1 + c.(tick);
-                                                    extr := 0 |}) c; |}.
-  Proof.
-    abstract (simpl; intuition; subst; eauto; [
-    rewrite <- cycle_irrelevance in *; eauto; rewrite <- H1; eauto |
-    rewrite <- cycle_irrelevance in *; eauto; rewrite H1; eauto ]).  Defined. *)
-
-  Record test :=
-    { a : FixInt 16;
-      b : FixInt 16;
-      c : { s : list (FixInt 16) | length s = 16 };
-      d : { s : list ascii | length s < exp2_nat 3 } }.
-
-  Definition et (e : test) :=
-         FixInt_encode (FixList_getlength e.(d))
-    Then FixInt_encode (e.(b))
-    Then FixInt_encode (e.(a))
-    Then IList_encode btransformer FixInt_encode e.(c)
-    Then FixList_encode btransformer Char_encode e.(d)
-    Done.
-  Set Printing Implicit. Print et. Unset Printing Implicit.
-  Instance edr
-    : decoder _ btransformer (fun _ => True) et.
-  Proof.
-         eapply compose_decoder.
-         solve_decoder.
-         instantiate (1:=fun _ => True). abstract intuition.
-         intro.
-         eapply compose_decoder.
-         solve_decoder.
-         instantiate (1:=fun _ => True). abstract intuition.
-         intro.
-         eapply compose_decoder.
-         solve_decoder.
-         instantiate (1:=fun _ => True). unfold IList_predicate. abstract intuition.
-         intro.
-         eapply compose_decoder.
-         solve_decoder.
-         solve_predicate.
-         intro.
-         eapply compose_decoder.
-         solve_decoder.
-         solve_predicate.
-         intro.
-         eexists (fun b e => (Build_test proj1 proj0 proj2 proj3, b, e)). abstract (
-
-                        intros ? ? ? ? hdata ? ? ? ? ? ? ?; destruct hdata; simpl in *;
-
-                        cbv beta; intros; repeat match goal with
-                        | [ H : (_, _) = (_, _) |- _ ] => inversion H; subst; clear H
-                        end; intuition; subst; eauto). Defined.
-
-  Definition ed b := fst (fst (decode (decoder:=edr) b empty)).
-  Definition ans2 := ed packet_uncompressed.
-
-  Goal True.
-    Set Printing Implicit.
-    pose ans2 as d.
-    unfold ans2, ed, edr in d.
-    simpl in d.
-  Abort.
-
-  Definition sample := fst (FixInt_decode 18 _ packet_uncompressed empty).
-  Goal True.
-    pose sample as d.
-    unfold sample, FixInt_decode in d.
-    simpl in d.
-  Abort.
-
-  Global Instance word_decoder
-    : decoder cache btransformer (fun _ => True) encode_word.
-  Proof. eapply compose_decoder.
-         eapply FixInt_decoder.
-         instantiate (1:=fun _ => True). abstract intuition.
-         intro.
-         eapply compose_decoder.
-         eapply FixList_decoder. eapply Char_decoder.
-         unfold FixList_predicate.
-         instantiate (2:=proj). instantiate (1:=fun _ => True). abstract intuition.
-         intro.
-         eexists (fun b e => (Build_word_t proj0, b, e)). abstract (
-
-                        intros ? ? ? ? hdata ? ? ? ? ? ? ?; destruct hdata; simpl in *;
-
-                        cbv beta; intros; repeat match goal with
-                        | [ H : (_, _) = (_, _) |- _ ] => inversion H; subst; clear H
-                        end; intuition; subst; eauto).
-  Defined.
-  Print word_decoder.
-  Definition word_decode b := fst (fst (decode (decoder:=word_decoder) b empty)).
-  Definition ans2 := word_decode packet_uncompressed.
-  Eval vm_compute in ans2.
-
-(*
-Definition p : packet_t.
-  refine ({| pid := exist _ (true :: true :: true :: true ::
-                             true :: true :: true :: true ::
-                             true :: true :: true :: true ::
-                             true :: true :: true :: true :: nil) _;
-             pmask := exist _ (true :: true :: true :: true ::
-                             true :: true :: true :: true ::
-                             true :: true :: true :: true ::
-                             true :: true :: true :: true :: nil) _;
-             pquestion := exist _ nil _;
-             panswer := exist _ nil _;
-             pauthority := exist _ nil _;
-             padditional := exist _ nil _ |}); admit.
-Defined.
-
-Lemma compose_decoder_decode A A'
-      (cache : Cache)
-      (transformer : Transformer)
-      (project : A -> A')
-      (predicate : A -> Prop)
-      (predicate' : A' -> Prop)
-      (encode1 : A' -> CacheEncode -> bin * CacheEncode)
-      (encode2 : A -> CacheEncode -> bin * CacheEncode)
-      (decoder1 : decoder cache transformer predicate' encode1)
-      (pred_pf : forall data, predicate data -> predicate' (project data))
-      (decoder2 : forall proj,
-          decoder cache transformer (fun data => predicate data /\ project data = proj) encode2)
-      (b : bin)
-      (cd : CacheDecode)
-  : decode (decoder:=(compose_decoder project predicate decoder1 pred_pf decoder2)) b cd =
-    let (bundle, env') := @decode _ _ _ _ _ decoder1 b cd in
-    let (proj, rest) := bundle in
-    @decode _ _ _ _ _ (decoder2 proj) rest env'.
-Proof. reflexivity.  Qed.
-
-Definition x (Tranformer:=btransformer) (b : bin) : packet_t * bin * CacheDecode.
-  pose (decode_packet_i b).
-  unfold decode_packet_i in p0.
-  cbv beta delta [ packet_decoder ] in p0.
-
-  let p0' := eval unfold p0 in p0 in
-  match p0' with
-  | context [ compose_decoder ?proj ?pred ?decoder1' ?pred_pf ?decoder2' ] =>
-    pose proof (compose_decoder_decode proj pred decoder1' pred_pf decoder2' b
-               ({| eMap := EMap.empty position_t;
-                   dMap := DMap.empty (list word_t);
-                   tick := 0;
-                   extr := 0 |})) (*
-    rewrite compose_decoder_decode with (decoder1:=decoder1') (decoder2:=decoder2') in p0 *)
-  end.
-  Set Printing Implicit. idtac.
-  unfold encode_packet in p0.
-  rewrite H in p0.
-
-  rewrite compose_decoder_decode in p0.
-
-  let p0 := eval unfold p0 in p0 in
-  match p0 with
-  | context [ compose_decoder ?pid ?pred ?decoder1 _ ?decoder2 ] => set (x:=decoder2) in *
-  end.
-  unfold compose_decoder in p0.
-
-  cbv beta delta [ decode ] in p0.
-  unfold IList_decoder in p0.
-  Opaque IList_decode. idtac. Set Printing Implicit. idtac. clearbody x.
-  simpl in p0.
-
-Eval vm_compute in (fst (encode_packet_i p)).
-(* Eval vm_compute in (decode_packet_i (fst (encode_packet_i p))). *)
-
-(*
-Global Instance test_decoder
-  : decoder test_cache btransformer (fun _ => True) encode_test.
-Proof.
-  unfold encode_test.
-
-  eapply compose_decoder; eauto with typeclass_instances; intuition.
-  instantiate (1:=fun _ => True); eauto.
-
-  eapply compose_decoder; eauto with typeclass_instances; intuition.
-  instantiate (1:=fun _ => True); eauto.
-
-  eapply compose_decoder; eauto with typeclass_instances; intuition.
-  instantiate (1:=fun _ => True); eauto.
-
-  eapply compose_decoder; eauto with typeclass_instances; intuition.
-  instantiate (1:=fun _ => True); eauto.
-
-  eexists. unfold encode_decode_correct.
-  instantiate (1:=fun b e => (Build_test_t proj proj0 proj1 proj2, b, e)).
-  intuition. inversion H1. inversion H2. subst. eauto. inversion H2.
-  subst. destruct data. eauto. inversion H1. subst. inversion H2. eauto.
-Defined. *)
-
-Section Examples.
-End Examples.
-
-
-
-Extract Inductive bool => "bool" [ "true" "false" ].
-Extract Inductive sumbool => "bool" [ "true" "false" ].
-Extract Inductive list => "list" [ "[]" "(::)" ].
-Extract Inductive prod => "(*)"  [ "(,)" ].
-Extract Inductive ascii => char [
-"(fun (b0,b1,b2,b3,b4,b5,b6,b7) -> let f b i = if b then 1 lsl i else 0 in Char.chr (f b0 0 + f b1 1 + f b2 2 + f b3 3 + f b4 4 + f b5 5 + f b6 6 + f b7 7))"
-]
-"(fun f c -> let n = Char.code c in let h i = (n land (1 lsl i)) <> 0 in f (h 0) (h 1) (h 2) (h 3) (h 4) (h 5) (h 6) (h 7))".
-
-Check DMap.Raw.Proofs.L.find_rect.
-Eval vm_compute in (fst (encode_packet_i p)).
-(* Extraction "p.ml" encode_packet_i encode_packet'_i p. *)*)
-
-
-(*
-Definition encode_word (w : word_t) :=
-  compose btransformer (FixInt_encode _ (FixList_getlength w.(word))) (
-  compose btransformer (FixList_encode _ btransformer (Char_encode _) w.(word))
-                       (fun e => (nil, e))).
-
-Definition encode_name (n : name_t) :=
-  compose btransformer
-          (SteppingList_encode _ _ _ btransformer encode_word (FixInt_encode _)
-                              (Enum_encode _ FixInt_of_branch) n.(name))
-          (fun e => (nil, e)).
-
-Definition encode_question (q : question_t) :=
-  compose btransformer (encode_name q.(qname)) (
-  compose btransformer (Enum_encode _ FixInt_of_type q.(qtype)) (
-  compose btransformer (Enum_encode _ FixInt_of_class q.(qclass))
-                       (fun e => (nil, e)))).
-
-Definition encode_resource (r : resource_t) :=
-  compose btransformer (encode_name r.(rname)) (
-  compose btransformer (Enum_encode _ FixInt_of_type r.(rtype)) (
-  compose btransformer (Enum_encode _ FixInt_of_class r.(rclass)) (
-  compose btransformer (FixInt_encode _ r.(rttl)) (
-  compose btransformer (FixInt_encode _ (FixList_getlength r.(rdata))) (
-  compose btransformer (FixList_encode _ btransformer (Bool_encode _) r.(rdata))
-                       (fun e => (nil, e))))))).
-
-Definition encode_packet (p : packet_t) :=
-  compose btransformer (IList_encode _ btransformer (Bool_encode _) p.(pid)) (
-  compose btransformer (IList_encode _ btransformer (Bool_encode _) p.(pmask)) (
-  compose btransformer (FixInt_encode _ (FixList_getlength p.(pquestion))) (
-  compose btransformer (FixInt_encode _ (FixList_getlength p.(panswer))) (
-  compose btransformer (FixInt_encode _ (FixList_getlength p.(pauthority))) (
-  compose btransformer (FixInt_encode _ (FixList_getlength p.(padditional))) (
-  compose btransformer (FixList_encode _ btransformer encode_question p.(pquestion)) (
-  compose btransformer (FixList_encode _ btransformer encode_resource p.(panswer)) (
-  compose btransformer (FixList_encode _ btransformer encode_resource p.(pauthority)) (
-  compose btransformer (FixList_encode _ btransformer encode_resource p.(padditional))
-                       (fun e => (nil, e))))))))))). *)
 *)
