src/BinEncoders/Env/Automation/Solver.v
@@ -38,7 +38,7 @@ Ltac idtac' :=
 
 Definition FixInt_eq_dec (size : nat) (n m : {n | (n < exp2 size)%N }) : {n = m} + {n <> m}.
   refine (if N.eq_dec (proj1_sig n) (proj1_sig m) then left _ else right _);
-    destruct n; destruct m; try congruence; simpl in *; rewrite <- sig_equivalence; eauto.
+    abstract (destruct n; destruct m; try congruence; simpl in *; rewrite <- sig_equivalence; eauto).
 Defined.
 
 Ltac solve_enum :=
